src/QUIC.Parse.fsti
@@ -1,8 +1,144 @@
 module QUIC.Parse
+include QUIC.Spec.Base
 
 module B = LowStar.Buffer
 module U8 = FStar.UInt8
 module U32 = FStar.UInt32
 module HST = FStar.HyperStack.ST
+module S = FStar.Seq
+module U64 = FStar.UInt64
 
+
+let header_len_bound = 16500 // FIXME: this should be in line with the parser kind
+
+val header_len (h:header) : GTot (n: pos { n <= header_len_bound })
+
+(*
+=
+  match h with
+  | MShort spin phase cid ->
+    1 + S.length cid + 1 + pn_len
+  | MLong is_hs version dcil scil dcid scid plen ->
+    let _ = assert_norm(max_cipher_length < pow2 62) in
+    6 + add3 dcil + add3 scil + vlen plen + 1 + pn_len
+*)
+
+(*
+  | Short _ _ cid -> sub3 (S.length cid)
+  | Long _ _ dcil _ _ _ _ -> dcil
+*)
+
+val format_header: h:header -> GTot (lbytes (header_len h))
+
+module BF = LowParse.BitFields
+
+val format_header_is_short: h: header -> Lemma
+  (MShort? h <==> BF.get_bitfield (U8.v (S.index (format_header h) 0)) 7 8 == 0)
+
+val format_header_is_retry: h: header -> Lemma
+  (is_retry h <==> (
+    BF.get_bitfield (U8.v (S.index (format_header h) 0)) 7 8 == 1 /\
+    BF.get_bitfield (U8.v (S.index (format_header h) 0)) 4 6 == 3
+  ))
+
+val format_header_pn_length: h: header -> Lemma
+  (requires (~ (is_retry h)))
+  (ensures (BF.get_bitfield (U8.v (S.index (format_header h) 0)) 0 2 == U32.v (pn_length h)))
+
+val pn_offset: (h: header { ~ (is_retry h) }) -> GTot (n: nat { 0 < n /\ n + U32.v (pn_length h) <= header_len h })
+
+val putative_pn_offset: (cid_len: nat) -> (x: bytes) -> GTot (option (y: nat {0 < y /\ y <= Seq.length x}))
+
+val putative_pn_offset_frame
+  (cid_len: nat)
+  (x1 x2: bytes)
+: Lemma
+  (requires (match putative_pn_offset cid_len x1 with
+  | None -> False
+  | Some off ->
+    off <= Seq.length x2 /\
+    Seq.slice x1 1 off `Seq.equal` Seq.slice x2 1 off /\ (
+    let f1 = Seq.index x1 0 in
+    let f2 = Seq.index x2 0 in
+    let is_short = BF.get_bitfield (U8.v f1) 7 8 = 0 in
+    let number_of_protected_bits = if is_short then 5 else 4 in
+    BF.get_bitfield (U8.v f1) number_of_protected_bits 8 == BF.get_bitfield (U8.v f2) number_of_protected_bits 8
+  )))
+  (ensures (match putative_pn_offset cid_len x1 with
+  | None -> False
+  | Some off -> putative_pn_offset cid_len x2 == Some (off <: nat)
+  ))
+
+val putative_pn_offset_correct
+  (h: header {~ (is_retry h)})
+  (cid_len: nat)
+: Lemma
+  (requires (MShort? h ==> cid_len == dcid_len h))
+  (ensures (putative_pn_offset cid_len (format_header h) == Some (pn_offset h <: nat)))
+
+noeq
+type h_result =
+| H_Success:
+  h: header ->
+  c: bytes ->
+  h_result
+| H_Failure
+
+val parse_header: cid_len: nat { cid_len < 20 } -> last: nat { last + 1 < pow2 62 } -> b:bytes -> GTot (r: h_result {
+  match r with
+  | H_Failure -> True
+  | H_Success h c ->
+    (MShort? h ==> dcid_len h == cid_len) /\
+    ((~ (is_retry h)) ==> in_window (U32.v (pn_length h) - 1) last (U64.v (packet_number h))) /\
+    Seq.length c <= Seq.length b /\
+    c == Seq.slice b (Seq.length b - Seq.length c) (Seq.length b)
+})
+
+val lemma_header_parsing_correct:
+  h: header ->
+  c: bytes ->
+  cid_len: nat { cid_len < 20 } ->
+  last: nat { last + 1 < pow2 62 } ->
+  Lemma
+  (requires (
+    (MShort? h ==> cid_len == dcid_len h) /\
+    ((~ (is_retry h)) ==> in_window (U32.v (pn_length h) - 1) last (U64.v (packet_number h)))
+  ))
+  (ensures (
+    parse_header cid_len last S.(format_header h @| c)
+    == H_Success h c))
+
+// N.B. this is only true for a given DCID len
+val lemma_header_parsing_safe: cid_len: nat -> last: nat -> b1:bytes -> b2:bytes -> Lemma
+  (requires (
+    cid_len < 20 /\
+    last + 1 < pow2 62 /\
+    parse_header cid_len last b1 == parse_header cid_len last b2
+  ))
+  (ensures parse_header cid_len last b1 == H_Failure \/ b1 = b2)
+
+let lemma_header_parsing_post
+  (cid_len: nat { cid_len < 20 })
+  (last: nat { last + 1 < pow2 62 })
+  (b: bytes)
+: Lemma
+  (match parse_header cid_len last b with
+  | H_Failure -> True
+  | H_Success h c ->
+    (MShort? h ==> dcid_len h == cid_len) /\
+    header_len h + Seq.length c == Seq.length b /\
+    b == format_header h `Seq.append` c /\
+    Seq.slice b 0 (header_len h) == format_header h /\
+    c == Seq.slice b (header_len h) (Seq.length b)
+  )
+= match parse_header cid_len last b with
+  | H_Failure -> ()
+  | H_Success h c ->
+    lemma_header_parsing_correct h c cid_len last ;
+    lemma_header_parsing_safe cid_len last b (format_header h `S.append` c);
+    assert (b `Seq.equal` (format_header h `Seq.append` c));
+    assert (Seq.slice b 0 (header_len h) `Seq.equal` format_header h);
+    assert (c `Seq.equal` Seq.slice b (header_len h) (Seq.length b))
+
+(*
 val test : B.buffer U8.t -> HST.Stack U32.t (requires (fun _ -> False)) (ensures (fun _ _ _ -> True))
