src/QUIC.Parse.PacketNumber.fst
@@ -1,0 +1,209 @@
+module QUIC.Parse.PacketNumber
+open QUIC.Spec.Base
+open QUIC.Parse.Lemmas
+open LowParse.Low.Combinators
+open LowParse.Low.BoundedInt
+
+(* From https://tools.ietf.org/html/draft-ietf-quic-transport-22#appendix-A *)
+
+module Cast = FStar.Int.Cast
+module U64 = FStar.UInt64
+module U32 = FStar.UInt32
+module U16 = FStar.UInt16
+module U8 = FStar.UInt8
+
+inline_for_extraction
+let bound_npn
+  (pn_len: packet_number_length_t)
+: Tot (x: U64.t { U64.v x == bound_npn' (U32.v pn_len - 1) })
+= if pn_len = 1ul
+  then 256uL
+  else if pn_len = 2ul
+  then 65536uL
+  else if pn_len = 3ul
+  then 16777216uL
+  else 4294967296uL
+
+let reduce_pn' pn_len pn = pn % (bound_npn' pn_len)
+
+inline_for_extraction
+let reduce_pn
+  (pn_len: packet_number_length_t)
+  (pn: uint62_t)
+: Tot (b: bounded_integer (U32.v pn_len) { U32.v b == reduce_pn' (U32.v pn_len - 1) (U64.v pn) })
+= [@inline_let]
+  let _ =
+    assert_norm (pow2 32 == 4294967296)
+  in
+  if pn_len = 4ul
+  then Cast.uint64_to_uint32 pn
+  else Cast.uint64_to_uint32 (pn `U64.rem` bound_npn pn_len)
+
+let in_window_self (pn_len: nat { pn_len < 4 }) (pn:nat) : Lemma
+  (in_window pn_len pn (if pn = 0 then 0 else pn - 1))
+= ()
+
+#push-options "--max_fuel 2 --initial_fuel 2 --max_ifuel 1 --initial_ifuel 1"
+let expand_pn'
+  (pn_len: nat { pn_len < 4 })
+  (last: nat { last + 1 < pow2 62})
+  (npn: nat { npn < bound_npn' pn_len })
+: Tot (pn: nat { pn < pow2 62 /\ in_window pn_len last pn /\ pn % bound_npn' pn_len == npn })
+=
+  let open FStar.Mul in
+  let open FStar.Math.Lemmas in
+  let expected = last + 1 in
+  let bound = bound_npn' pn_len in
+  let candidate = replace_modulo' expected bound npn in
+  lemma_replace_modulo_bound expected (8*(pn_len+1)) npn 62;
+  if candidate <= last + 1 - bound/2
+     && candidate < pow2 62 - bound then // the test for overflow (candidate < pow2 62 - bound) is not present in draft 22.
+    let _ = lemma_mod_plus candidate 1 bound in
+    candidate + bound
+  else if candidate > last + 1 + bound/2
+          && candidate >= bound then // in draft 22 the test for underflow (candidate >= bound) uses a strict inequality, which makes it impossible to expand npn to 0
+    let _ = lemma_mod_plus candidate (-1) bound in
+    candidate - bound
+  else candidate
+#pop-options
+
+let max (a b:int) : Tot (n:int{n >= a /\ n >= b}) =
+  if a > b then a else b // this must exist somewhere...
+
+let lemma_uniqueness_in_window (pn_len: nat { pn_len < 4 }) (last: nat { last < pow2 62 }) (x: nat {x < pow2 62}) (y:nat {y < pow2 62}) : Lemma
+  (requires (
+    let h = bound_npn' pn_len in
+    in_window pn_len last x /\
+    in_window pn_len last y /\
+    x%h = y%h))
+  (ensures x = y) =
+  let open FStar.Math.Lemmas in
+  pow2_lt_compat 62 (8 `op_Multiply` (pn_len+1));
+  let h = bound_npn' pn_len in
+  if last+1 < h/2 && x < h then
+    lemma_mod_plus_injective h 0 x y
+  else if last+1 >= pow2 62 - h/2 && x >= pow2 62 - h then
+    let low = pow2 62 - h in
+    lemma_mod_plus_injective h low (x-low) (y-low)
+  else
+    let low = max (last+2-h/2) 0 in
+    lemma_mod_plus_injective h low (x-low) (y-low)
+
+val lemma_parse_pn_correct : (pn_len: nat { pn_len < 4 }) -> last:nat{last+1 < pow2 62} -> (pn: nat { pn < U64.v uint62_bound }) -> Lemma
+  (requires in_window pn_len last pn)
+  (ensures expand_pn' pn_len last (reduce_pn' pn_len pn) = pn)
+
+let lemma_parse_pn_correct pn_len last pn =
+  lemma_uniqueness_in_window pn_len last pn (expand_pn' pn_len last (reduce_pn' pn_len pn))
+
+#push-options "--max_fuel 2 --initial_fuel 2 --max_ifuel 1 --initial_ifuel 1 --z3rlimit 64"
+
+let expand_pn
+  (pn_len: packet_number_length_t)
+  (last: last_packet_number_t)
+  (npn: bounded_integer (U32.v pn_len))
+: Tot (pn: uint62_t { U64.v pn == expand_pn' (U32.v pn_len - 1) (U64.v last) (U32.v npn) })
+= let open FStar.Mul in
+  let open FStar.Math.Lemmas in
+  let expected : uint62_t = last `U64.add` 1uL in
+  let bound = bound_npn pn_len in
+  let candidate = replace_modulo expected bound (Cast.uint32_to_uint64 npn) in
+  if (bound `U64.div` 2uL) `U64.lte` expected
+     && candidate `U64.lte` (expected `U64.sub` (bound `U64.div` 2uL))
+     && candidate `U64.lt` (uint62_bound `U64.sub` bound) then // the test for overflow (candidate < pow2 62 - bound) is not present in draft 22.
+//    let _ = lemma_mod_plus candidate 1 bound in
+    candidate `U64.add` bound
+  else if candidate `U64.gt` (expected `U64.add` (bound `U64.div` 2uL))
+          && candidate `U64.gte` bound then // in draft 22 the test for underflow (candidate >= bound) uses a strict inequality, which makes it impossible to expand npn to 0
+//    let _ = lemma_mod_plus candidate (-1) bound in
+    candidate `U64.sub` bound
+  else candidate
+#pop-options
+
+inline_for_extraction
+let synth_packet_number
+  (last: last_packet_number_t)
+  (pn_len: packet_number_length_t)
+  (npn: bounded_integer (U32.v pn_len))
+: Tot (pn: packet_number_t last pn_len { U64.v pn == expand_pn' (U32.v pn_len - 1) (U64.v last) (U32.v npn) })
+= expand_pn pn_len last npn
+
+let parse_packet_number
+  (last: last_packet_number_t)
+  (pn_len: packet_number_length_t)
+: Tot (parser (parse_bounded_integer_kind (U32.v pn_len)) (packet_number_t last pn_len) )
+= parse_bounded_integer (U32.v pn_len) `parse_synth` synth_packet_number last pn_len
+
+inline_for_extraction
+let synth_packet_number_recip
+  (last: last_packet_number_t)
+  (pn_len: packet_number_length_t)
+  (pn: packet_number_t last pn_len)
+: Tot  (bounded_integer (U32.v pn_len))
+= reduce_pn pn_len pn
+
+let synth_packet_number_recip_inverse
+  (last: last_packet_number_t)
+  (pn_len: packet_number_length_t)
+: Lemma
+  (synth_inverse (synth_packet_number last pn_len) (synth_packet_number_recip last pn_len))
+//  [SMTPat (synth_inverse (synth_packet_number last pn_len) (synth_packet_number_recip last pn_len))] // TODO: WHY WHY WHY does this pattern not trigger?
+= synth_inverse_intro' #(bounded_integer (U32.v pn_len)) #(packet_number_t last pn_len) (synth_packet_number last pn_len) (synth_packet_number_recip last pn_len) (fun pn ->
+    lemma_parse_pn_correct (U32.v pn_len - 1) (U64.v last) (U64.v pn)
+  )
+
+let serialize_packet_number
+  (last: last_packet_number_t)
+  (pn_len: packet_number_length_t)
+: Tot (serializer (parse_packet_number last pn_len))
+= synth_packet_number_recip_inverse last pn_len;
+  serialize_synth
+    _
+    (synth_packet_number last pn_len)
+    (serialize_bounded_integer (U32.v pn_len))
+    (synth_packet_number_recip last pn_len)
+    ()
+
+#push-options "--z3rlimit 16"
+
+let serialize_packet_number_ext
+  (last1 last2: last_packet_number_t)
+  (pn_len: packet_number_length_t)
+  (pn: uint62_t)
+: Lemma
+  (requires (
+    in_window (U32.v pn_len - 1) (U64.v last1) (U64.v pn) /\
+    in_window (U32.v pn_len - 1) (U64.v last2) (U64.v pn)
+  ))
+  (ensures (
+    in_window (U32.v pn_len - 1) (U64.v last1) (U64.v pn) /\
+    in_window (U32.v pn_len - 1) (U64.v last2) (U64.v pn) /\
+    serialize (serialize_packet_number last1 pn_len) pn == serialize (serialize_packet_number last2 pn_len) pn
+  ))
+= synth_packet_number_recip_inverse last1 pn_len;
+  synth_packet_number_recip_inverse last2 pn_len;
+  serialize_synth_eq 
+    _
+    (synth_packet_number last1 pn_len)
+    (serialize_bounded_integer (U32.v pn_len))
+    (synth_packet_number_recip last1 pn_len)
+    ()
+    pn;
+  serialize_synth_eq 
+    _
+    (synth_packet_number last2 pn_len)
+    (serialize_bounded_integer (U32.v pn_len))
+    (synth_packet_number_recip last2 pn_len)
+    ()
+    pn
+
+#pop-options
+
+let validate_packet_number
+  (last: last_packet_number_t)
+  (pn_len: packet_number_length_t)
+: Tot (validator (parse_packet_number last pn_len))
+= validate_synth
+    (validate_bounded_integer (U32.v pn_len))
+    (synth_packet_number last pn_len)
+    ()
