src/QUIC.Parse.PacketNumber.fsti
@@ -1,0 +1,37 @@
+module QUIC.Parse.PacketNumber
+open QUIC.Spec.Base
+open LowParse.Low.Base
+
+module Cast = FStar.Int.Cast
+module U64 = FStar.UInt64
+module U32 = FStar.UInt32
+module U16 = FStar.UInt16
+module U8 = FStar.UInt8
+
+inline_for_extraction
+let parse_packet_number_kind
+  (sz: packet_number_length_t)
+: Tot parser_kind
+= total_constant_size_parser_kind (U32.v sz)
+
+inline_for_extraction
+let packet_number_t
+  (last: last_packet_number_t)
+  (pn_len: packet_number_length_t)
+: Tot eqtype
+= (pn: uint62_t { in_window (U32.v pn_len - 1) (U64.v last) (U64.v pn) })
+
+val parse_packet_number
+  (last: last_packet_number_t)
+  (pn_len: packet_number_length_t)
+: Tot (parser (parse_packet_number_kind pn_len) (packet_number_t last pn_len))
+
+val serialize_packet_number
+  (last: last_packet_number_t)
+  (pn_len: packet_number_length_t)
+: Tot (serializer (parse_packet_number last pn_len))
+
+val validate_packet_number
+  (last: last_packet_number_t)
+  (pn_len: packet_number_length_t)
+: Tot (validator (parse_packet_number last pn_len))
