src/QUIC.Spec.Base.fst
@@ -1,0 +1,139 @@
+module QUIC.Spec.Base
+
+module FB = FStar.Bytes
+module U64 = FStar.UInt64
+module U32 = FStar.UInt32
+module U8 = FStar.UInt8
+module S = FStar.Seq
+
+inline_for_extraction
+let uint62_bound : (uint62_bound: U64.t { U64.v uint62_bound == pow2 62 }) =
+  [@inline_let] let v = 4611686018427387904uL in
+  [@inline_let] let _ = assert_norm (U64.v v == pow2 62) in
+  v
+
+inline_for_extraction
+let uint62_t = (x: U64.t { U64.v x < U64.v uint62_bound })
+
+type byte = FStar.UInt8.t
+type bytes = s:S.seq byte
+type lbytes (n:nat) = b:bytes{S.length b = n}
+
+inline_for_extraction
+let vlbytes (min: nat) (max: nat) =
+  (x: FB.bytes { min <= FB.length x /\ FB.length x <= max })
+
+inline_for_extraction
+noextract
+let token_max_len = 16383 // arbitrary bound
+
+inline_for_extraction
+noextract
+type packet_number_length_t : eqtype = (x: U32.t { 1 <= U32.v x /\ U32.v x <= 4 })
+
+inline_for_extraction
+noextract
+let bitfield
+  (sz: nat { sz <= 8 })
+: Tot eqtype
+= (x: U8.t { U8.v x < pow2 sz })
+
+noeq
+type long_header_specifics =
+| MInitial:
+  (token: vlbytes 0 token_max_len) -> // arbitrary bound
+  (payload_length: uint62_t) ->
+  (packet_number_length: packet_number_length_t) ->
+  (packet_number: uint62_t) ->
+  long_header_specifics
+| MZeroRTT:
+  (payload_length: uint62_t) ->
+  (packet_number_length: packet_number_length_t) ->
+  (packet_number: uint62_t) ->
+  long_header_specifics
+| MHandshake:
+  (payload_length: uint62_t) ->
+  (packet_number_length: packet_number_length_t) ->
+  (packet_number: uint62_t) ->
+  long_header_specifics
+| MRetry:
+  (unused: bitfield 4) ->
+  (odcid: vlbytes 0 20) -> // TODO: change bounds to drop instead of rejecting as invalid
+  long_header_specifics
+
+noeq
+type header =
+| MLong:
+  (version: FB.lbytes 4) ->
+  (dcid: vlbytes 0 20) ->
+  (scid: vlbytes 0 20) ->
+  (spec: long_header_specifics) ->
+  header
+| MShort:
+  (spin: bool) ->
+  (key_phase: bool) ->
+  (dcid: vlbytes 0 20) ->
+  (packet_number_length: packet_number_length_t) ->
+  (packet_number: uint62_t) ->
+  header
+
+let is_initial (h: header) : Tot bool =
+  if MLong? h then MInitial? (MLong?.spec h) else false
+
+let is_zero_rtt (h: header) : Tot bool =
+  if MLong? h then MZeroRTT? (MLong?.spec h) else false
+
+let is_handshake (h: header) : Tot bool =
+  if MLong? h then MHandshake? (MLong?.spec h) else false
+
+let is_retry (h: header) : Tot bool =
+  if MLong? h then MRetry? (MLong?.spec h) else false
+
+let pn_length (h: header { ~ (is_retry h) }) : Tot packet_number_length_t =
+  match h with
+  | MLong _ _ _ spec ->
+    begin match spec with
+    | MInitial _ _ pnl _ -> pnl
+    | MZeroRTT _ pnl _ -> pnl
+    | MHandshake _ pnl _ -> pnl
+    end
+  | MShort _ _ _ pnl _ -> pnl
+
+let packet_number (h: header {~ (is_retry h)}) : Tot uint62_t =
+  match h with
+  | MLong _ _ _ spec ->
+    begin match spec with
+    | MInitial _ _ _ pn -> pn
+    | MZeroRTT _ _ pn -> pn
+    | MHandshake _ _ pn -> pn
+    end
+  | MShort _ _ _ _ pn -> pn
+
+let dcid_len (h: header) : Tot nat =
+  match h with
+  | MLong _ dcid _ _ -> FB.length dcid
+  | MShort _ _ dcid _ _ -> FB.length dcid
+
+type packet = b:bytes{let l = S.length b in (* 21 <= l /\ *) l < pow2 32}
+
+(* Packet number *)
+
+inline_for_extraction
+let last_packet_number_t = (last: uint62_t { U64.v last + 1 < U64.v uint62_bound})
+
+let bound_npn' (pn_len:nat { pn_len < 4 }) : Tot (y: nat {y == pow2 (8 `op_Multiply` (pn_len + 1)) }) =
+  assert_norm (pow2 8 == 256);
+  assert_norm (pow2 16 == 65536);
+  assert_norm (pow2 24 == 16777216);
+  assert_norm (pow2 32 == 4294967296);
+  match pn_len with
+  | 0 -> 256
+  | 1 -> 65536
+  | 2 -> 16777216
+  | 3 -> 4294967296
+
+let in_window (pn_len: nat { pn_len < 4 }) (last pn:nat) =
+  let h = bound_npn' pn_len in
+  (last+1 < h/2 /\ pn < h) \/
+  (last+1 >= U64.v uint62_bound - h/2 /\ pn >= U64.v uint62_bound - h) \/
+  (last+1 - h/2 < pn /\ pn <= last+1 + h/2)
